Rewrite the interpreters to use the state monad

Soundness.v
@@ -7,149 +7,12 @@ Require Import AbstractStore.
 Require Import AbstractInterpreter.
 Require Import Aux.
 Require Import ConcreteInterpreter.
+Require Import Galois.
+Require Import Language.
+Require Import Maps.
 Require Import Parity.
 Require Import Preorder.
-Require Import Maps.
-Require Import Language.
-
 Open Scope com_scope.
-
-Lemma abstract_aexp_plus_sound : forall e1 e2,
-  sound_aexp e1 ->
-  sound_aexp e2 ->
-  sound_aexp (APlus e1 e2).
-Proof. 
-  unfold sound_aexp. intros. simpl. apply parity_plus_sound. 
-  apply H. assumption.
-  apply H0. assumption.
-Qed.
-
-Lemma abstract_aexp_mult_sound : forall e1 e2,
-  sound_aexp e1 ->
-  sound_aexp e2 ->
-  sound_aexp (AMult e1 e2).
-Proof.
-  unfold sound_aexp. intros. apply parity_mult_sound. apply H. assumption.
-  apply H0. assumption. Qed.
-
-Lemma abstract_aexp_var_sound : forall x,
-  sound_aexp (AVar x).
-Proof. intros. unfold sound_aexp. intros. simpl. unfold sound_store in H.
-  apply H. Qed.
-
-Theorem abstract_aexp_eval_sound : forall e,
-  sound_aexp e.
-Proof. 
-  induction e; intros.
-  - (* ANum *) unfold sound_aexp. intros. simpl. apply gamma_extract_n_n.
-  - (* AVar *) apply abstract_aexp_var_sound. 
-  - (* APlus *) apply abstract_aexp_plus_sound; auto.
-  - (* AMult *) apply abstract_aexp_mult_sound; auto.
-Qed.
-
-Lemma abstract_beval_eq_sound : forall a1 a2,
-  sound_bexp (BEq a1 a2).
-Proof.
-  unfold sound_bexp. intros. 
-  unfold sound_ab. apply parity_eq_sound.
-  apply abstract_aexp_eval_sound. assumption. apply abstract_aexp_eval_sound.
-  assumption.
-Qed.
-
-Theorem abstract_beval_sound : forall e,
-  sound_bexp e.
-Proof. 
-  unfold sound_bexp. intros. induction e.
-  - reflexivity. 
-  - simpl. tauto. 
-  - apply abstract_beval_eq_sound. assumption. 
-  - reflexivity.
-  - simpl. apply neg_ab_sound. assumption.
-  - simpl. apply and_ab_sound. assumption. assumption.
-Qed.
-
-Lemma abstract_ceval_ass_sound : forall y a,
-  sound_com (y ::= a).
-Proof.
-  unfold sound_com. 
-  intros. simpl. unfold t_update, sound_store. intros.
-  destruct (beq_string y x). 
-  - apply abstract_aexp_eval_sound. apply H.
-  - unfold sound_store in H. apply H.
-Qed.
-
-Lemma abstract_ceval_seq_sound : forall c1 c2,
-  sound_com c1 ->
-  sound_com c2 ->
-  sound_com (c1 ;; c2).
-Proof. 
-  unfold sound_com. intros. apply H0. apply H. assumption.
-Qed.
-
-Lemma abstract_ceval_if_sound : forall b c1 c2,
-  sound_com c1 ->
-  sound_com c2 ->
-  sound_com (CIf b c1 c2).
-Proof. 
-  unfold sound_com. intros. simpl. 
-  pose proof abstract_beval_sound. unfold sound_bexp in H2. 
-  assert (sound_ab (beval_abstract ast b) (eval_bexp st b)).
-  { apply H2. assumption. }
-  destruct (eval_bexp st b), (beval_abstract ast b);
-    unfold sound_ab, gamma_bool, not in H3; try inversion H3.
-  - apply H; assumption.
-  - exfalso. apply H3. reflexivity.
-  - simpl. apply abstract_store_join_sound_left. auto.
-  - simpl. auto. 
-  - simpl. apply abstract_store_join_sound_right. auto.
-Qed.
-
-Theorem abstract_ceval_sound : forall c,
-  sound_com c.
-Proof. 
-  intros c. induction c; intros.
-  - (* SKIP *) unfold sound_com. simpl. intros. assumption.
-  - (* CSeq *) apply abstract_ceval_seq_sound; assumption.
-  - apply abstract_ceval_ass_sound.
-  - apply abstract_ceval_if_sound; assumption.
-Qed.
-
-Record IsGalois {A B} (g : B -> A -> Prop)  
-                      (e : A->B)
-                      (j : B->B->B) 
-                      (o : B->B->Prop) :=
-{
-}.
-
-
-Class Galois (A B : Type) `{PreorderedSet A} `{PreorderedSet B} : Type :=
-{
-  gamma : B -> A -> Prop;
-  gamma_monotone : forall b b', preorder b b' -> preorder (gamma b) (gamma b');  
-}.
-Arguments Build_Galois A B {_ _ _ _}.
-Arguments gamma {_ _ _ _ _}.
-
-Instance galois_self {A :Type} `{PreorderedSet A} : Galois A A :=
-{
-  gamma := fun _ _ => True;
-}.
-- intros b b' H'. simpl. constructor.  reflexivity.
-Defined.
-(* 
-Discuss with Sven
-
-- Add an extract function to the galois definition?
-- Definition of soundness
-
-- forall n, gamma (extract n) n.
-  *)
-
-Lemma test : forall {X : Type} (P Q : X -> Prop) (x : X),
-  preorder P Q -> P x -> Q x.
-Proof. 
-  intros. simpl in H. destruct H. apply H. apply H0.
-Qed.
 
 Instance galois_parity_nat : Galois nat parity :=
 {
@@ -181,12 +44,12 @@ Lemma widen {A A' B:Type} `{Galois B A'}:
   forall (f1 f2 : A->A') (x:A) (a:B),
   pointwise_ordering f1 f2 -> gamma (f1 x) a -> gamma (f2 x) a.
 Proof. 
-  intros. apply test with (P:=(gamma (f1 x))) 
+  intros. 
+  apply preorder_props with (P:=(gamma (f1 x))) 
     (Q:=(gamma (f2 x))). 
     - apply gamma_monotone. destruct H2. apply H2.
     - apply H3.
 Qed.
-
 
 Definition gamma_fun {A A' B B' : Type} `{Galois B A} `{Galois B' A'} : 
   (A->A') -> (B -> B') -> Prop :=
