Galois.v
@@ -1,0 +1,25 @@
+Require Import Preorder.
+
+Record IsGalois {A B} (g : B -> A -> Prop)  
+                      (e : A->B)
+                      (j : B->B->B) 
+                      (o : B->B->Prop) :=
+{
+}.
+
+
+Class Galois (A B : Type) `{PreorderedSet A} `{PreorderedSet B} : Type :=
+{
+  gamma : B -> A -> Prop;
+  gamma_monotone : forall b b', preorder b b' -> preorder (gamma b) (gamma b');  
+}.
+Arguments Build_Galois A B {_ _ _ _}.
+Arguments gamma {_ _ _ _ _}.
+
+Instance galois_self {A :Type} `{PreorderedSet A} : Galois A A :=
+{
+  gamma := fun _ _ => True;
+}.
+- intros b b' H'. simpl. constructor.  reflexivity.
+Defined.
+
