Monad.v
@@ -1,16 +1,14 @@
-Require Import AbstractStore.
+Definition State {S : Type} (A : Type) := S -> (A * S)%type.
 
+Definition return_state {A S : Type} (x : A) : State A :=
+  fun (st : S) => (x, st).
 
-Definition State (A : Type) := store -> (A * store)%type.
-
-Definition return_state {A : Type} (x : A) : State A :=
-  fun (st : store) => (x, st).
-
-Definition bind_state {A B : Type} (m : State A) (f : A -> State B) : State B :=
+Definition bind_state {S A B : Type} (m : @State S A) (f : A -> @State S B) 
+    : State B :=
   fun st => let (x, st') := (m st) in f x st'.
 
-Definition get : State store := fun st => (st, st).
+Definition get {S : Type} : State S := fun st => (st, st).
 
-Definition put (st' : store) : State unit := fun st => (tt, st).
+Definition put {S : Type} (st' : S) : @State S unit := fun st => (tt, st').
  
 
